Adapt txn proof

src/program_proof/mvcc/txnmgr_repr.v
@@ -7,7 +7,7 @@ Context `{!heapGS Σ, !mvcc_ghostG Σ}.
 (* TODO: Rename [tidsactiveM]. *)
 Definition own_txnsite (txnsite : loc) (sid : u64) γ : iProp Σ := 
   ∃ (tidsactive : Slice.t) (tidsactiveL : list u64) (tidsactiveM : gset nat),
-    "Hactive" ∷ txnsite ↦[TxnSite :: "tidsActive"] (to_val tidsactive) ∗
+    "Hactive" ∷ txnsite ↦[TxnSite :: "tids"] (to_val tidsactive) ∗
     "HactiveL" ∷ typed_slice.own_slice tidsactive uint64T 1 tidsactiveL ∗
     "HactiveAuth" ∷ site_active_tids_half_auth γ sid tidsactiveM ∗
     (* "%HactiveLM" ∷ ⌜(∀ tid, tid ∈ (int.Z <$> tidsactiveL) ↔ tid ∈ (Z.of_nat <$> (elements tidsactiveM)))⌝ ∗ *)
@@ -23,7 +23,7 @@ Definition is_txnsite (site : loc) (sid : u64) γ : iProp Σ :=
 
 Definition own_txnmgr (txnmgr : loc) : iProp Σ := 
   ∃ (sidcur : u64),
-    "Hsidcur" ∷ txnmgr ↦[TxnMgr :: "sidCur"] #sidcur ∗
+    "Hsidcur" ∷ txnmgr ↦[TxnMgr :: "sid"] #sidcur ∗
     "%HsidcurB" ∷ ⌜(int.Z sidcur) < N_TXN_SITES⌝ ∗
     "_" ∷ True.
 
@@ -38,7 +38,7 @@ Definition is_txnmgr (txnmgr : loc) γ : iProp Σ :=
     "#HsitesS" ∷ readonly (own_slice_small sites ptrT 1 (to_val <$> sitesL)) ∗
     "%HsitesLen" ∷ ⌜Z.of_nat (length sitesL) = N_TXN_SITES⌝ ∗
     "#HsitesRP" ∷ ([∗ list] sid ↦ site ∈ sitesL, is_txnsite site sid γ) ∗
-    "#Hp" ∷ readonly (txnmgr ↦[TxnMgr :: "p"] #p) ∗
+    "#Hp" ∷ readonly (txnmgr ↦[TxnMgr :: "proph"] #p) ∗
     "#Hinvgc" ∷ mvcc_inv_gc γ ∗
     "#Hinvsst" ∷ mvcc_inv_sst γ p ∗
     "#Hinvtid" ∷ have_gentid γ ∗
